Some cleanup

pico-invsubtyping-limitedvpa/ViewpointAdaptation.v
@@ -10,13 +10,6 @@ Definition vpa_mutabilty_qq (q1: q)(q2 : q) : q :=
 
 (* A wrapper around vpa_mutability by taking two full types *)
 Definition vpa_mutabilty_tt (t1: qualified_type)(t2 : qualified_type) : qualified_type :=
-  (* let abs_result := 
-    match (sabs t1), (sabs t2) with
-    | Protected, _ => Protected
-    | _, Protected => Protected
-    | Normal, Normal => Normal
-    end
-  in *)
   let qual_result :=
     match (sqtype t1), (sqtype t2) with
     | RO, RDM => Lost
